Define unification with its termination proof. Whew!

Traat/chapter2.lean
@@ -1,5 +1,6 @@
 import Traat.chapter1
 import Mathlib.Data.Finset.Basic
+import Mathlib.Data.Finset.Card
 
 -- We're going to define an applicative version of terms.
 -- We don't parametrize on vars or signature, a specific
@@ -15,6 +16,7 @@ inductive Term where
 | var : Var → Term
 | func : Sig → Term
 | app : Term → Term → Term
+deriving DecidableEq
 
 open Term
 
@@ -32,13 +34,20 @@ abbrev Subst := Var → Term
 
 -- The domain of a substitution is the set of variables
 -- which are *not* sent to themselves.
-def dom (σ : Subst) (x : Var) : Prop := σ x ≠ var x
+def Subst.dom (σ : Subst) : Set Var := { x | σ x ≠ var x }
 
 def Term.apply (t : Term) (σ : Subst) : Term :=
   match t with
   | var v => σ v
   | t₁ @@ t₂ => t₁.apply σ @@ t₂.apply σ
   | _ => t
+
+-- We compose substitutions in the "inverse" order, that is,
+-- the opposite of what `∘` does (but the natural order for arrows)
+def Subst.scomp (σ : Subst) (τ : Subst) : Subst :=
+  fun x => (σ x).apply τ
+
+abbrev Subst.idSubst : Subst := var
 
 #check Finset.disjUnion_eq_union
 #check Finset.instUnion
@@ -55,7 +64,11 @@ def Term.sig : Term → Finset Sig
 | t₁ @@ t₂ => t₁.sig ∪ t₂.sig
 | _ => {}
 
+@[grind =_]
+lemma Term.subst_id (t : Term) : t = t.apply Subst.idSubst := by induction t <;> grind [Term.apply]
+
 -- Ok let's define equations, and formalize deduction.
+section Equational
 
 structure FormalEq where
   lhs : Term
@@ -65,6 +78,7 @@ infix:29 " ≅ " => FormalEq.mk
 
 #check "f" @@ var "x" ≅ "g" @@ var "x"
 
+open Subst
 
 -- Sometimes it's useful to not have variables
 -- in application position
@@ -104,12 +118,12 @@ infix:25 " ⊢ " => Derives
 -- pretty much all of rewrite theory.
 @[grind]
 inductive Derives : Ctxt → FormalEq → Prop where
-| ax : E ∈ Γ → Γ ⊢ E
+| ax : (t ≅ u) ∈ Γ → Γ ⊢ t ≅ u
 | refl : Γ ⊢ (t ≅ t)
 | symm : Γ ⊢ (t ≅ u) → Γ ⊢ (u ≅ t)
 | trans : Γ ⊢ (t ≅ u) → Γ ⊢ (u ≅ v) → Γ ⊢ (t ≅ v)
 | congr : Γ ⊢ t₁ ≅ t₂ → Γ ⊢ u₁ ≅ u₂ → Γ ⊢ t₁ @@ u₁ ≅ t₂ @@ u₂
-| inst : Γ ⊢ (t ≅ u) → Γ ⊢ (t.apply σ ≅ u.apply σ)
+| subst : Γ ⊢ (t ≅ u) → Γ ⊢ (t.apply σ ≅ u.apply σ)
 
 #check {} ⊢ "f" @@ var "x" ≅ "f" @@ var "x"
 
@@ -193,9 +207,9 @@ lemma subst_eval [M : Model ℳ] (θ : Valuation ℳ) σ t : ⦃t.apply σ⦄ θ
 
 theorem soundness : Γ ⊢ E → Γ ⊧ E := by
   intros h; induction h
-  case _ E h =>
+  case _ t u h =>
     simp; intros _ _ h' θ
-    apply h'; trivial
+    apply h' ⟨t, u⟩; trivial
   case _ => simp only [models, Model.models, Ctxt.satisfies, FormalEq.satisfies, FormalEq.eval,
     implies_true]
   case _ h' =>
@@ -259,8 +273,6 @@ lemma subst_term_model (Γ : Ctxt) (t : Term) (σ : Subst) :
     rw [← ih₁, ← ih₂]
     simp only [Model.app, Quotient.map₂_mk]
 
-lemma subst_id (t : Term) : t = t.apply (fun x => var x) := by induction t <;> grind [Term.apply]
-
 #check Quotient.out
 #check Quotient.out_eq
 
@@ -276,8 +288,295 @@ theorem completeness (Γ : Ctxt) (E : FormalEq) : Γ ⊧ E → Γ ⊢ E := by
     intros E mem θ
     rw [← subst_lift]; rw [← subst_lift, Quotient.eq_iff_equiv]
     simp [HasEquiv.Equiv, SetoidCtx, CtxtRel]
-    apply Derives.inst; apply Derives.ax; exact mem
+    apply Derives.subst; apply Derives.ax; exact mem
   have models := models (TermModel Γ) h (fun x => ⟦var x⟧); simp at models
   rw [← subst_term_model] at models
   rw [← subst_term_model, Quotient.eq_iff_equiv, ← subst_id] at models
   rw [← subst_id] at models; exact models
+
+end Equational
+
+-- on to rewriting! Not that different.
+section Rewriting
+
+structure Rule where
+  lhs : Term
+  rhs : Term
+
+abbrev Rules := Set Rule
+
+open Subst
+-- This is not quite rewriting logic, since we'll only have
+-- congruence and not all the relfexive transitive stuff.
+@[grind]
+inductive Reduces (ℛ : Rules) : Term → Term → Prop where
+| ax : ⟨l, r⟩ ∈ ℛ → Reduces ℛ l r
+| congr : Reduces ℛ t₁ t₂ → Reduces ℛ u₁ u₂ → Reduces ℛ (t₁ @@ u₁) (t₂ @@ u₂)
+| subst : Reduces ℛ t u → Reduces ℛ (t.apply σ) (u.apply σ)
+
+-- Let's fix a rewrite system
+variable (ℛ : Rules)
+
+abbrev RTerm (_ℛ : Rules) := Term
+
+instance termRed : Red (RTerm ℛ) where
+  reduces := Reduces ℛ
+
+#check termRed
+-- set_option trace.Meta.synthInstance true
+#synth Red (RTerm ℛ)
+
+-- This is a little depressing: We can't just use `Term` here to get the notation.
+#check fun (t u : RTerm ℛ) => t ~> u
+
+#check let t : RTerm ℛ := "f" @@ var "x"; let u : RTerm ℛ := "g" @@ var "x"; t ~> u
+
+-- Test lemma
+lemma Test.idRed (t : RTerm ℛ) : t ~>* t := by simp [Red.reduces]; grind
+
+def UnifyProp (t u : Term) : Prop := ∃ σ, t.apply σ = u.apply σ
+
+def varUnify (x : Var) (t : Term) : Option Subst :=
+  if x ∈ t.vars then none else (fun y => if y = x then t else var y)
+
+@[grind =]
+lemma varUnify_some_iff (x : Var) (t : Term) : (varUnify x t).isSome ↔ x ∉ t.vars := by grind [varUnify]
+
+@[grind .]
+lemma varsSubApply₁ (t₁ t₂ : Term) : t₁.vars ⊆ (t₁ @@ t₂).vars := by
+  simp [Term.vars]
+
+@[grind .]
+lemma varsSubApply₂ (t₁ t₂ : Term) : t₂.vars ⊆ (t₁ @@ t₂).vars := by
+  simp [Term.vars]
+
+lemma substDom (t : Term) (σ τ : Subst) (h : ∀ x ∈ t.vars, σ x = τ x) : t.apply σ = t.apply τ := by
+  induction t <;> simp [Term.apply, Term.vars] at * <;> grind only
+
+lemma varDom (t : Term) (σ : Subst) (h : Disjoint σ.dom t.vars) : t.apply σ = t := by
+  have h' : t = t.apply idSubst := by grind
+  have h'' : ∀ x ∈ t.vars, σ x = idSubst x := by
+    intros x; simp [idSubst]
+    rw [Set.disjoint_right] at h
+    simp [dom] at h
+    apply h
+  grind [substDom]
+
+
+lemma varUnifyDom (x : Var) (t : Term) (h : varUnify x t |>.isSome) :
+  (varUnify x t |>.get h).dom ⊆ {x} := by
+  simp [dom, varUnify]
+
+lemma varUnifyUnif (x : Var) (t : Term) (h : varUnify x t |>.isSome) :
+  (varUnify x t).get h x = t.apply ((varUnify x t).get h) := by
+  have h₁ : x ∉ t.vars := by
+    simp [varUnify] at h; trivial
+  have h₂ : Disjoint ((varUnify x t).get h).dom t.vars := by
+    grind [varUnifyDom]
+  rw [varDom]; simp [varUnify]; trivial
+
+lemma varUnifyMGU  (x : Var) (t : Term) (σ : Subst)
+  (unifies : varUnify x t |>.isSome)
+  (hasUnifier : σ x = t.apply σ)
+: let mgu := varUnify x t |>.get unifies
+  ∃ τ : Subst, mgu.scomp τ = σ := by
+  simp [varUnify]
+  exists (fun y => if y = x then t.apply σ else σ y)
+  funext y
+  by_cases h:(y = x); simp [h, scomp]
+  . rw [substDom t _ σ] <;> grind
+  . simp [scomp, h, Term.apply]
+
+#print Decidable
+#print DecidableEq
+
+#synth DecidableEq Term
+
+instance domDec {σ : Subst} {x : Var} : Decidable (x ∈ σ.dom) :=
+  if h : σ x = var x then .isFalse (by simp [dom]; exact h) else .isTrue h
+
+@[simp]
+def Subst.join (σ₁ σ₂ : Subst) : Subst :=
+  fun x => if x ∈ σ₁.dom then σ₁ x else σ₂ x
+
+lemma joinDisjCommut (σ₁ σ₂ : Subst) (disj : Disjoint σ₁.dom σ₂.dom) : σ₁.join σ₂ = σ₂.join σ₁ := by
+  funext x; simp
+  by_cases h : (x ∈ σ₁.dom)
+  . simp [Set.disjoint_left] at *
+    grind
+  . simp [h]
+    simp [dom] at *; grind
+
+
+structure UnifyState where
+  subst : Subst
+  constraints : List (Term × Term)
+
+def constrVars : List (Term × Term) → Finset Var
+| [] => {}
+| (t, u) :: cs => t.vars ∪ u.vars ∪ (constrVars cs)
+
+def Subst.map₂ (σ : Subst) (l : List (Term × Term)) : List (Term × Term) :=
+  l.map (fun (x, y) => (x.apply σ, y.apply σ))
+
+lemma substCodom (t : Term) (σ : Subst) (codom_inc : ∀ x ∈ t.vars, (σ x).vars ⊆ S) :
+  (t.apply σ).vars ⊆ S := by
+  induction t <;> simp [Term.apply, Term.vars] <;> simp [Term.vars] at codom_inc <;> grind
+
+lemma excludeCodom (t : Term) (σ : Subst) (x : Var) (h : ∀ y, x ∉ (σ y).vars) : x ∉ (t.apply σ).vars := by
+  induction t <;> simp [apply, vars] <;> grind
+
+lemma substMapDom (l : List (Term × Term)) (σ : Subst)
+  (codom_inc : ∀ x ∈ constrVars l, (σ x).vars ⊆ S) :
+  constrVars (σ.map₂ l) ⊆ S := by
+  revert codom_inc; induction l <;> simp [constrVars, Subst.map₂]
+  case _ head tail ih =>
+    intros codom_inc
+    rw [Finset.union_subset_iff]; rw [Finset.union_subset_iff]
+    apply And.intro
+    . grind [substCodom]
+    . apply And.intro; grind [substCodom]
+      apply ih; grind
+
+lemma excludeConstrCodom (l : List (Term × Term)) (σ : Subst) (x : Var) (h : ∀ y, x ∉ (σ y).vars) : x ∉ constrVars (σ.map₂ l) := by
+  induction l <;> simp [Subst.map₂, constrVars]
+  case _ t₁ t₂ ih =>
+    have h' := fun t => excludeCodom t σ x h
+    exact ⟨h' _, h' _, ih⟩ -- why doesn't grind work here?
+
+def unifyStep (st : UnifyState) : Option UnifyState :=
+  match st.constraints with
+  | [] => none -- kind of a hack to fail here, but we won't hit this branch.
+  | (func f, func g) :: cstr =>
+    if f = g then
+      return ⟨st.subst, cstr⟩
+    else failure
+  | (var x, t) :: cstr => do
+    let σ ← varUnify x t
+    let newConstr := σ.map₂ cstr
+    return ⟨σ.join st.subst, newConstr⟩
+  | (t, var x) :: cstr => do
+    let σ ← varUnify x t
+    let newConstr := cstr.map (fun (x, y) => (x.apply σ, y.apply σ))
+    return ⟨σ.join st.subst, newConstr⟩
+  | (t₁ @@ u₁, t₂ @@ u₂) :: cstr => do
+    return ⟨st.subst, (t₁, t₂) :: (u₁, u₂) :: cstr⟩
+  | (_, _) :: _ => failure
+
+#synth SizeOf (List ℕ)
+
+#print List._sizeOf_1
+
+#print Term._sizeOf_1
+
+noncomputable def constrSize : List (Term × Term) → ℕ
+| [] => 0
+| (t₁, t₂) :: cstrs => 1 + sizeOf t₁ + sizeOf t₂ + (constrSize cstrs)
+
+noncomputable def ltState (st : UnifyState) : ℕ × ℕ :=
+  (constrVars st.constraints |> Finset.card, constrSize st.constraints)
+
+#print Prod.Lex
+
+lemma cardExcludedMem α (s s' : Finset α) (x : α) :
+  s ≤ s' → x ∈ s' → x ∉ s → s.card < s'.card := by
+  simp; intros; apply Finset.card_lt_card; grind
+
+@[grind →]
+lemma unifyStep_isSome_var
+  (h : (unifyStep { subst := subst, constraints := (var x, u) :: tail }).isSome) :
+  (varUnify x u).isSome := by
+  revert h; simp [unifyStep, Option.bind]
+  split <;> grind
+
+-- This is the clever bit: we get rid of a variable with that `varUnify`,
+-- which decreases the second leg of the measure.
+private lemma constrRemoveVar (h : (varUnify x u).isSome) :
+  (constrVars (((varUnify x u).get h).map₂ tail)).card <
+  (insert x (u.vars ∪ constrVars tail)).card := by
+  apply cardExcludedMem (x := x)
+  . have vu_some : (varUnify x u).isSome := by grind
+    have h' := substMapDom (S := u.vars ∪ constrVars tail) tail (varUnify x u |>.get vu_some)
+    apply Finset.Subset.trans (s₂ := u.vars ∪ constrVars tail)
+    . apply h'
+      intros y h
+      by_cases eq:(y = x)
+      . rw [eq]; simp [varUnify]
+      . simp [varUnify, eq, Term.vars]
+        grind
+    . simp
+  . grind
+  . have vu_some : (varUnify x u).isSome := by grind
+    apply excludeConstrCodom
+    intros y; by_cases h':(y = x)
+    . simp [h', varUnify]; grind
+    . simp [varUnify, h', Term.vars]; grind
+
+-- This is quite a bit more tedious than I'd like.
+lemma decltState : Prod.Lex (· < ·) (· < ·)
+  (ltState ((unifyStep st).get h)) (ltState st) := by
+  have ⟨_, l⟩ := st
+  cases l <;> simp [unifyStep]
+  case nil => simp [unifyStep] at h
+  -- These are just a single deconstruction, there's gotta be a better way.
+  case cons hd tail =>
+  cases hd
+  case _ t u =>
+  --------------
+  cases t
+  case _ x =>
+    apply Prod.Lex.left; simp [constrVars, Term.vars]
+    apply constrRemoveVar
+  case _ =>
+    cases u
+    case _ f x =>
+      apply Prod.Lex.left; simp [constrVars, Term.vars]
+      have h' := constrRemoveVar (x:=x) (tail:=tail) (u := func f)
+      simp [Subst.map₂, Term.vars] at h'
+      apply h'
+    case _ =>
+      apply Prod.Lex.right' <;> simp [constrVars]
+      . apply Finset.card_mono
+        simp [LE.le]; grind
+      . simp [constrSize]
+    case _ => simp [unifyStep] at h
+  case _ t₁ t₂ =>
+    cases u
+    case _ x =>
+      apply Prod.Lex.left; simp [constrVars, Term.vars]
+      have h' := constrRemoveVar (x:=x) (tail:=tail) (u := t₁ @@ t₂)
+      simp [Subst.map₂, Term.vars] at h'
+      apply h'
+    case _ => simp [unifyStep] at h
+    case _ =>
+      apply Prod.Lex.right' <;> simp [constrVars]
+      . apply Finset.card_mono
+        simp [LE.le, Term.vars]; grind
+      . simp [constrSize]; grind
+
+def unify_aux (st : UnifyState) : Option Subst :=
+  match st.constraints with
+  | [] => return st.subst
+  | _ =>
+    -- We can't use pretty do notation here to not confuse the termination
+    -- checker
+    let st' := unifyStep st
+    if h: st'.isSome then unify_aux (st'.get h) else none
+  termination_by ltState st
+  decreasing_by
+    apply decltState
+
+-- This is the "simple" version, but proving termination is quite hard.
+partial def unify' (t₁ t₂ : Term) : Option Subst :=
+  match t₁, t₂ with
+  | func f, func g => if f = g then idSubst else none
+  | var x, t => varUnify x t
+  | t, var x => varUnify x t
+  | t₁ @@ u₁, t₂ @@ u₂ =>
+    do
+      let σ₁ ← unify' t₁ t₂
+      let σ₂ ← unify' (u₁.apply σ₁) (u₂.apply σ₁)
+      return σ₁.join σ₂
+  | _, _ => none
+
+end Rewriting
